updates to the bootstrap
mainly for the reorganised compsets

also replace compile_primitives with prim_env

bootstrap/compile_repl_decsScript.sml
@@ -1,20 +1,24 @@
-open HolKernel boolLib bossLib cakeml_computeLib ml_repl_moduleTheory compile_primitivesTheory flookupLib
+open HolKernel boolLib bossLib ml_repl_moduleTheory flookupLib compute_compilerLib
 val _ = new_theory"compile_repl_decs"
 
 val compile_repl_decs_def = zDefine`
-  compile_repl_decs = compile_top NONE (FST compile_primitives) (Tmod "REPL" NONE ml_repl_module_decls)`
+  compile_repl_decs = compile_top NONE ((FST(THE prim_env)).comp_rs) (Tmod "REPL" NONE ml_repl_module_decls)`
 
 val _ = Globals.max_print_depth := 20
 
-val cs = cakeml_compset();
+val cs = the_compiler_compset false;
 (*TODO: add FUNION_FUPDATE_1 to finite_map compset*)
-val _ = computeLib.add_thms [finite_mapTheory.FUNION_FUPDATE_1,compile_primitives_eq] cs
-val _ = computeLib.scrub_const cs finite_mapSyntax.flookup_t;
-val _ = computeLib.add_conv (finite_mapSyntax.flookup_t,2,FLOOKUP_DEFN_CONV) cs;
+val () = computeLib.add_thms [finite_mapTheory.FUNION_FUPDATE_1] cs
+val () = computeLib.scrub_const cs finite_mapSyntax.flookup_t;
+val () = computeLib.add_conv (finite_mapSyntax.flookup_t,2,FLOOKUP_DEFN_CONV) cs;
+(* TODO: this should go into a separate compset *)
+val () = computeLib.add_datatype_info cs (valOf(TypeBase.fetch``:comp_environment``))
 val eval = computeLib.CBV_CONV cs
 
 val compile_repl_decs_eq = save_thm("compile_repl_decs_eq",
-  time (REWR_CONV compile_repl_decs_def THENC PURE_ONCE_REWRITE_CONV[ml_repl_module_decls] THENC eval)
+  time (REWR_CONV compile_repl_decs_def
+        THENC PURE_ONCE_REWRITE_CONV[ml_repl_module_decls,initCompEnvTheory.prim_env_eq]
+        THENC eval)
   ``compile_repl_decs``)
 
 val repl_decs_code_def = zDefine
@@ -29,8 +33,7 @@ val call_dec = ``Tdec (Dlet (Plit Unit) (App Opapp [Var(Long"REPL""call_repl_ste
 val compile_call_repl_step_def = zDefine`
   compile_call_repl_step = compile_special (FST compile_repl_decs) ^call_dec`
 
-
-val _ = computeLib.add_thms [compilerProofTheory.compile_special_def] cs
+val _ = computeLib.add_thms [compilerTheory.compile_special_def] cs
 val eval_special = computeLib.CBV_CONV cs
 val compile_call_repl_step_eq = save_thm("compile_call_repl_step_eq",
   time (REWR_CONV compile_call_repl_step_def THENC
@@ -42,8 +45,9 @@ val compile_call_repl_step_labels = store_thm("compile_call_repl_step_labels",
   ``FILTER is_Label compile_call_repl_step = []``,
   REWRITE_TAC[compile_call_repl_step_eq] THEN EVAL_TAC)
 
+val eval_fvs = computeLib.CBV_CONV (the_free_vars_compset())
 val FV_decs_ml_repl_module_decls = save_thm("FV_decs_ml_repl_module_decls",
-  time (PURE_ONCE_REWRITE_CONV[ml_repl_module_decls] THENC eval)
+  time (PURE_ONCE_REWRITE_CONV[ml_repl_module_decls] THENC eval_fvs)
   ``FV_decs ml_repl_module_decls``)
 
 val _ = Feedback.set_trace "TheoryPP.include_docs" 0
